iris/UkShRun.v
@@ -392,7 +392,7 @@ Section UkShRun.
     WP (Loop : expr riscv_lang).
   Proof.
     intros Hns He1 He2 Ha Hal Hrd. iIntros "#Hi Hw Hrun Hcont".
-    iDestruct "Hrun" as (C pt Rfd Rut sz M pm fdv) "(%Hlo & %Hpm & Hheap & Hstk & Hb)".
+    iDestruct "Hrun" as (xi C pt Rfd Rut sz M pm fdv) "(%Hlo & %Hpm & Hheap & Hstk & Hb)".
     iDestruct (uinstr_is_uk_instr with "Hheap Hi") as %Hui.
     iDestruct (uheap_access γt γd γs M pm dq a 8 (nth_byte w)
                  ltac:(lia) ltac:(right; right; right; reflexivity) Hal
@@ -435,7 +435,7 @@ Section UkShRun.
     WP (Loop : expr riscv_lang).
   Proof.
     intros Hns He1 He2 Ha Hal Hrd. iIntros "#Hi Hw Hrun Hcont".
-    iDestruct "Hrun" as (C pt Rfd Rut sz M pm fdv) "(%Hlo & %Hpm & Hheap & Hstk & Hb)".
+    iDestruct "Hrun" as (xi C pt Rfd Rut sz M pm fdv) "(%Hlo & %Hpm & Hheap & Hstk & Hb)".
     iDestruct (uinstr_is_uk_instr with "Hheap Hi") as %Hui.
     iDestruct (uheap_access γt γd γs M pm dq a 4 (nth_byte wv)
                  ltac:(lia) ltac:(right; right; left; reflexivity) Hal
@@ -476,7 +476,7 @@ Section UkShRun.
     WP (Loop : expr riscv_lang).
   Proof.
     intros Hns Ha Hal Hrd. iIntros "#Hi Hw Hrun Hcont".
-    iDestruct "Hrun" as (C pt Rfd Rut sz M pm fdv) "(%Hlo & %Hpm & Hheap & Hstk & Hb)".
+    iDestruct "Hrun" as (xi C pt Rfd Rut sz M pm fdv) "(%Hlo & %Hpm & Hheap & Hstk & Hb)".
     iDestruct (uinstr_is_uk_instr with "Hheap Hi") as %Hui.
     iDestruct (uheap_access γt γd γs M pm dq a 4 (nth_byte wv)
                  ltac:(lia) ltac:(right; right; left; reflexivity) Hal
@@ -520,7 +520,7 @@ Section UkShRun.
     WP (Loop : expr riscv_lang).
   Proof.
     intros Hns He1 He2 Ha Hal Hrd. iIntros "#Hi #Hw Hrun Hcont".
-    iDestruct "Hrun" as (C pt Rfd Rut sz M pm fdv) "(%Hlo & %Hpm & Hheap & Hstk & Hb)".
+    iDestruct "Hrun" as (xi C pt Rfd Rut sz M pm fdv) "(%Hlo & %Hpm & Hheap & Hstk & Hb)".
     iDestruct (uinstr_is_uk_instr with "Hheap Hi") as %Hui.
     iDestruct (uheap_text_run γt γd γs M pm a 4%nat wv with "Hheap Hw")
       as %Hmap.
